floyd/SeparationLogicAsLogic.v
@@ -10,6 +10,7 @@ Require Export VST.veric.juicy_extspec.
 Require Import VST.veric.NullExtension.
 Require Import VST.floyd.val_lemmas VST.floyd.assert_lemmas.
 Require Import VST.floyd.SeparationLogicFacts.
+Require Import VST.floyd.FusionExact.
 Import LiftNotation.
 Import compcert.lib.Maps.
 Import Ctypes LiftNotation.
@@ -237,7 +238,7 @@ Inductive semax {CS: compspecs} {Espec: OracleKind} (Delta: tycontext): (environ
         (Sset id e) (normal_ret_assert P)
 | semax_store_store_union_hack_backward: forall (P: environ->mpred) e1 e2,
     @semax CS Espec Delta
-       ((EX sh: share, !! writable_share sh &&
+       (((EX sh: share, !! writable_share sh &&
              |> ( (tc_lvalue Delta e1) &&  (tc_expr Delta (Ecast e2 (typeof e1)))  &&
              ((`(mapsto_ sh (typeof e1)) (eval_lvalue e1)) *
               (`(mapsto sh (typeof e1)) (eval_lvalue e1) (`force_val (`(sem_cast (typeof e2) (typeof e1)) (eval_expr e2))) -* P))))
@@ -255,7 +256,7 @@ Inductive semax {CS: compspecs} {Espec: OracleKind} (Delta: tycontext): (environ
                     imp (local  ((`decode_encode_val )
                          ((` force_val) ((`(sem_cast (typeof e2) (typeof e1))) (eval_expr e2))) (`ch) (`ch') (`v') ))
                       (P)))))
-       )
+        ) || exact_store_pre Delta e1 e2 P)
         (Sassign e1 e2) (normal_ret_assert P)
 | semax_skip: forall P, @semax CS Espec Delta P Sskip (normal_ret_assert P)
 | semax_builtin: forall P opt ext tl el, @semax CS Espec Delta FF (Sbuiltin opt ext tl el) P
@@ -519,8 +520,8 @@ Qed.
 Lemma semax_assign_inv: forall {CS: compspecs} {Espec: OracleKind} Delta e1 e2 P Q,
   @semax CS Espec Delta P (Sassign e1 e2) Q ->
   local (tc_environ Delta) && (allp_fun_id Delta && P) |--
-     |={Ensembles.Full_set}=>
-      ((EX sh: share, !! writable_share sh &&
+      |={Ensembles.Full_set}=>
+       (((EX sh: share, !! writable_share sh &&
              |> ( (tc_lvalue Delta e1) &&  (tc_expr Delta (Ecast e2 (typeof e1)))  &&
              ((`(mapsto_ sh (typeof e1)) (eval_lvalue e1)) *
               (`(mapsto sh (typeof e1)) (eval_lvalue e1) (`force_val (`(sem_cast (typeof e2) (typeof e1)) (eval_expr e2))) -* |={Ensembles.Full_set}=> RA_normal Q))))
@@ -537,14 +538,19 @@ Lemma semax_assign_inv: forall {CS: compspecs} {Espec: OracleKind} Delta e1 e2 P
                  `(mapsto sh t2) (eval_lvalue e1) (`v') -*
                     imp (local  ((`decode_encode_val )
                          ((` force_val) ((`(sem_cast (typeof e2) (typeof e1))) (eval_expr e2))) (`ch) (`ch') (`v') ))
-                      (|={Ensembles.Full_set}=> RA_normal Q)))))
-       ).
+                       (|={Ensembles.Full_set}=> RA_normal Q)))))
+       ) || exact_store_pre Delta e1 e2 (|={Ensembles.Full_set}=> RA_normal Q)).
 Proof.
   intros.
   remember (Sassign e1 e2) as c eqn:?H.
   induction H; try solve [inv H0].
   + inv H0.
     reduce2derives.
+    apply orp_derives; [| unfold exact_store_pre;
+      do 2 (apply exp_derives; intro);
+      apply andp_derives; [auto |]; apply later_derives;
+      apply andp_derives; [auto |]; apply sepcon_derives; [auto |];
+      apply wand_derives; [auto |]; apply fupd_intro].
     apply orp_derives.
     - apply exp_derives; intro sh.
       apply andp_derives; auto.
@@ -569,6 +575,14 @@ Proof.
     derives_rewrite -> H.
     derives_rewrite -> (IHsemax eq_refl).
     reduceR.
+    apply orp_ENTAILL; [| unfold exact_store_pre;
+      do 2 (apply exp_ENTAILL; intro);
+      apply andp_ENTAILL; [reduceLL; apply ENTAIL_refl |];
+      apply later_ENTAILL;
+      apply andp_ENTAILL; [reduceLL; apply ENTAIL_refl |];
+      apply sepcon_ENTAILL; [reduceLL; apply ENTAIL_refl |];
+      apply wand_ENTAILL; [reduceLL; apply ENTAIL_refl |];
+      apply derives_full_fupd_left, H1].
     apply orp_ENTAILL.
     - apply exp_ENTAILL; intro sh.
       apply andp_ENTAILL; [reduceLL; apply ENTAIL_refl |].
@@ -1331,7 +1345,31 @@ Module Sassign: CLIGHT_SEPARATION_HOARE_LOGIC_SASSIGN_BACKWARD with Module CSHL_
 
 Module CSHL_Def := DeepEmbeddedDef.
 
-Definition semax_store_store_union_hack_backward := @AuxDefs.semax_store_store_union_hack_backward.
+Lemma semax_store_store_union_hack_backward:
+  forall {CS: compspecs} {Espec: OracleKind} Delta (P: environ -> mpred) e1 e2,
+    @semax CS Espec Delta
+      ((EX sh: share, !! writable_share sh &&
+        |> (tc_lvalue Delta e1 && tc_expr Delta (Ecast e2 (typeof e1)) &&
+          ((`(mapsto_ sh (typeof e1)) (eval_lvalue e1)) *
+           (`(mapsto sh (typeof e1)) (eval_lvalue e1)
+             (`force_val (`(sem_cast (typeof e2) (typeof e1)) (eval_expr e2))) -* P))))
+       || (EX (t2: type) (ch ch': memory_chunk) (sh: share),
+         !! ((numeric_type (typeof e1) && numeric_type t2)%bool = true /\
+             access_mode (typeof e1) = By_value ch /\
+             access_mode t2 = By_value ch' /\
+             decode_encode_val_ok ch ch' /\ writable_share sh) &&
+         |> (tc_lvalue Delta e1 && tc_expr Delta (Ecast e2 (typeof e1)) &&
+           ((`(mapsto_ sh (typeof e1)) (eval_lvalue e1) &&
+             `(mapsto_ sh t2) (eval_lvalue e1)) *
+            (ALL v': val, `(mapsto sh t2) (eval_lvalue e1) (`v') -*
+              imp (local ((`decode_encode_val)
+                ((`force_val) ((`(sem_cast (typeof e2) (typeof e1))) (eval_expr e2)))
+                (`ch) (`ch') (`v'))) P)))))
+      (Sassign e1 e2) (normal_ret_assert P).
+Proof.
+  intros. eapply semax_pre; [| apply AuxDefs.semax_store_store_union_hack_backward].
+  apply andp_left2, orp_right1, derives_refl.
+Qed.
 
 End Sassign.
 
@@ -1346,6 +1384,41 @@ Module StoreB := Sassign2Store (DeepEmbeddedDef) (Conseq) (Sassign).
 Module StoreF := StoreB2F (DeepEmbeddedDef) (Conseq) (StoreB).
 
 Definition semax_store := @StoreF.semax_store_forward.
+
+Lemma exact_store_backward:
+  forall {CS: compspecs} {Espec: OracleKind} Delta e1 e2 P,
+    @semax CS Espec Delta (exact_store_pre Delta e1 e2 P)
+      (Sassign e1 e2) (normal_ret_assert P).
+Proof.
+  intros. eapply semax_pre; [| apply AuxDefs.semax_store_store_union_hack_backward].
+  apply andp_left2, orp_right2, derives_refl.
+Qed.
+
+Theorem semax_store_exact:
+  forall {CS: compspecs} {Espec: OracleKind} (Delta: tycontext)
+    e1 e2 sh ch (P: environ -> mpred),
+    writable_share sh ->
+    access_mode (typeof e1) = By_value ch ->
+    @semax CS Espec Delta
+      (|> (tc_lvalue Delta e1 && tc_expr Delta (Ecast e2 (typeof e1)) &&
+        ((fun rho => mapsto_ sh (typeof e1) (eval_lvalue e1 rho)) * P)))
+      (Sassign e1 e2)
+      (normal_ret_assert
+        ((fun rho => exact_mapsto sh ch
+          (force_val (sem_cast (typeof e2) (typeof e1) (eval_expr e2 rho)))
+          (eval_lvalue e1 rho)) * P)).
+Proof.
+  intros.
+  eapply semax_pre; [| apply exact_store_backward].
+  unfold exact_store_pre.
+  apply (exp_right sh), (exp_right ch).
+  apply andp_right; [apply prop_right; auto |].
+  apply andp_left2, later_derives.
+  apply andp_derives; auto.
+  apply sepcon_derives; auto.
+  apply wand_sepcon_adjoint.
+  rewrite sepcon_comm; apply derives_refl.
+Qed.
 
 Definition semax_skip := @AuxDefs.semax_skip.
 
@@ -1637,6 +1710,15 @@ Proof.
       * apply ENTAIL_refl.
       * apply ENTAIL_refl.
   + eapply semax_pre; [| apply AuxDefs.semax_store_store_union_hack_backward].
+    apply orp_ENTAIL; [| unfold exact_store_pre;
+      do 2 (apply exp_ENTAIL; intro);
+      apply andp_ENTAIL; [apply ENTAIL_refl |];
+      apply later_ENTAIL; apply andp_ENTAIL; [| apply ENTAIL_refl];
+      apply andp_ENTAIL;
+      unfold local, lift1; intro rho; simpl; normalize;
+      constructor; [apply Clight_assert_lemmas.tc_lvalue_sub |
+                    apply Clight_assert_lemmas.tc_expr_sub]; auto;
+      eapply semax_lemmas.typecheck_environ_sub; eauto].
     apply orp_ENTAIL.
     - apply exp_ENTAIL; intro sh.
       apply andp_ENTAIL; [apply ENTAIL_refl |].
@@ -1767,7 +1849,7 @@ Definition SETpre CS Delta id e P :=
           @subst mpred id (` (force_val (sem_cast (typeof e1) t1 v2))) P)).
 
 Definition ASSIGNpre (CS: compspecs) Delta e1 e2 P: environ -> mpred :=
-  (EX sh : share,
+  ((EX sh : share,
            !! writable_share sh &&
            |> (tc_lvalue Delta e1 && tc_expr Delta (Ecast e2 (typeof e1)) &&
                ((` (mapsto_ sh (typeof e1))) (eval_lvalue e1) *
@@ -1788,7 +1870,7 @@ Definition ASSIGNpre (CS: compspecs) Delta e1 e2 P: environ -> mpred :=
                       ((` decode_encode_val)
                          ((` force_val)
                             ((` (sem_cast (typeof e2) (typeof e1))) (eval_expr e2)))
-                         (` ch) (` ch') (` v'))) P)))) .
+                          (` ch) (` ch') (` v'))) P))))) || @exact_store_pre CS Delta e1 e2 P.
 
 Definition STOREpre CS Delta e1 e2 P := (EX sh : share,
      !! writable_share sh &&
@@ -2022,6 +2104,26 @@ Proof.
   + apply semax_pre with (andp (ASSIGNpre CS Delta e1 e2 P) (ASSIGNpre CS' Delta e1 e2 P)).
     - intros rho. simpl. apply derives_extract_prop; intros TEDelta.
       apply andp_right. apply derives_refl. unfold ASSIGNpre; simpl.
+      apply orp_derives; [| unfold exact_store_pre; simpl;
+        apply exp_derives; intro sh; apply exp_derives; intro ch;
+        normalize; apply later_derives;
+        apply andp_right;
+        [apply andp_left1; apply andp_derives;
+          [apply tc_lvalue_cspecs_sub | apply tc_expr_cspecs_sub]; trivial |]] .
+      2: {
+        apply derives_trans with
+          ((!! (@eval_lvalue CS e1 rho = @eval_lvalue CS' e1 rho) &&
+            !! (@eval_expr CS e2 rho = @eval_expr CS' e2 rho)) &&
+           (mapsto_ sh (typeof e1) (@eval_lvalue CS e1 rho) *
+            (exact_mapsto sh ch
+              (force_val (sem_cast (typeof e2) (typeof e1) (@eval_expr CS e2 rho)))
+              (@eval_lvalue CS e1 rho) -* P rho))).
+        - apply andp_derives; [apply andp_derives | trivial].
+          + apply lvalue_cspecs_sub; trivial.
+          + eapply derives_trans. 2: apply rvalue_cspecs_sub; eassumption.
+            unfold tc_expr; simpl; rewrite denote_tc_assert_andp; simpl; solve_andp.
+        - normalize. rewrite H0, H1; trivial.
+      }
       apply orp_derives.
       *
         apply exp_derives; intros sh. normalize. apply later_derives.
@@ -2349,6 +2451,28 @@ Proof.
     eapply semax_pre; [| apply AuxDefs.semax_store_store_union_hack_backward].
     apply andp_left2.
     rewrite distrib_orp_sepcon.
+    apply orp_derives; [| unfold exact_store_pre;
+      rewrite exp_sepcon1; apply exp_derives; intro sh;
+      rewrite exp_sepcon1; apply exp_derives; intro ch;
+      normalize;
+      eapply derives_trans; [apply sepcon_derives; [apply derives_refl |]; apply now_later |];
+      rewrite <- later_sepcon; apply later_derives;
+      apply andp_right].
+    2: {
+      eapply derives_trans; [apply sepcon_derives; [| apply derives_refl]; apply andp_left1, derives_refl |].
+      intro rho; simpl; constructor.
+      apply (predicates_sl.extend_sepcon (extend_tc.extend_andp _ _
+        (extend_tc.extend_tc_lvalue Delta e1 rho)
+        (extend_tc.extend_tc_expr Delta (Ecast e2 (typeof e1)) rho))).
+    }
+    2: {
+      eapply derives_trans; [apply sepcon_derives; [| apply derives_refl]; apply andp_left2, derives_refl |].
+      rewrite sepcon_assoc; apply sepcon_derives; auto.
+      rewrite <- (emp_wand F) at 1.
+      eapply derives_trans; [apply wand_frame_hor |].
+      apply wand_derives; [rewrite sepcon_emp; auto | auto].
+    }
+    rewrite distrib_orp_sepcon.
     apply orp_derives.
     - rewrite exp_sepcon1; apply exp_derives; intros sh.
       normalize.
@@ -2648,6 +2772,9 @@ eapply @semax_adapt
 Qed.
 
 End DeepEmbeddedMinimumSeparationLogic.
+
+Definition exact_store_backward := @DeepEmbeddedMinimumSeparationLogic.exact_store_backward.
+Definition semax_store_exact := @DeepEmbeddedMinimumSeparationLogic.semax_store_exact.
 
 Module DeepEmbeddedPracticalLogic <: PRACTICAL_CLIGHT_SEPARATION_HOARE_LOGIC.
 
@@ -3264,4 +3391,3 @@ Definition semax_adapt := @DeepEmbeddedMinimumSeparationLogic.semax_adapt.
 End DeepEmbeddedPracticalLogic.
 
 End DeepEmbedded.
-
