floyd/FusionExact.v
@@ -1,0 +1,28 @@
+Require Import VST.veric.SeparationLogic.
+Require Import compcert.common.Memdata.
+
+Import Clight expr2.
+Local Open Scope Z.
+Local Open Scope logic.
+
+Definition exact_address_mapsto
+    (sh : share) (ch : memory_chunk) (v : val) (a : address) : mpred :=
+  !! (align_chunk ch | snd a) &&
+  res_predicates.address_mapsto_old ch v sh a.
+
+Definition exact_mapsto
+    (sh : share) (ch : memory_chunk) (v p : val) : mpred :=
+  match p with
+  | Vptr b ofs => exact_address_mapsto sh ch v (b, Ptrofs.unsigned ofs)
+  | _ => FF
+  end.
+
+Definition exact_store_pre {CS : compspecs} (Delta : tycontext)
+    (e1 e2 : expr) (P : environ -> mpred) : environ -> mpred :=
+  EX sh : share, EX ch : memory_chunk,
+  !! (writable_share sh /\ access_mode (typeof e1) = By_value ch) &&
+  |> (tc_lvalue Delta e1 && tc_expr Delta (Ecast e2 (typeof e1)) &&
+    ((fun rho => mapsto_ sh (typeof e1) (eval_lvalue e1 rho)) *
+     ((fun rho => exact_mapsto sh ch
+       (force_val (sem_cast (typeof e2) (typeof e1) (eval_expr e2 rho)))
+       (eval_lvalue e1 rho)) -* P))).
