fusion/tests/fusion_store.v
@@ -1,0 +1,1 @@
+Require Export VST.floyd.FusionStore.
