fusion/tests/seed_union_rw.v
@@ -1,0 +1,678 @@
+From Coq Require Import String List ZArith.
+From compcert Require Import Coqlib Integers Floats AST Ctypes Cop Clight Clightdefs.
+Import Clightdefs.ClightNotations.
+Local Open Scope Z_scope.
+Local Open Scope string_scope.
+Local Open Scope clight_scope.
+
+Module Info.
+  Definition version := "3.17".
+  Definition build_number := "".
+  Definition build_tag := "".
+  Definition build_branch := "".
+  Definition arch := "x86".
+  Definition model := "64".
+  Definition abi := "standard".
+  Definition bitsize := 64.
+  Definition big_endian := false.
+  Definition source_file := "fixtures/seed_union_rw.c".
+  Definition normalized := true.
+End Info.
+
+Definition ___builtin_ais_annot : ident := $"__builtin_ais_annot".
+Definition ___builtin_annot : ident := $"__builtin_annot".
+Definition ___builtin_annot_intval : ident := $"__builtin_annot_intval".
+Definition ___builtin_bswap : ident := $"__builtin_bswap".
+Definition ___builtin_bswap16 : ident := $"__builtin_bswap16".
+Definition ___builtin_bswap32 : ident := $"__builtin_bswap32".
+Definition ___builtin_bswap64 : ident := $"__builtin_bswap64".
+Definition ___builtin_clz : ident := $"__builtin_clz".
+Definition ___builtin_clzl : ident := $"__builtin_clzl".
+Definition ___builtin_clzll : ident := $"__builtin_clzll".
+Definition ___builtin_ctz : ident := $"__builtin_ctz".
+Definition ___builtin_ctzl : ident := $"__builtin_ctzl".
+Definition ___builtin_ctzll : ident := $"__builtin_ctzll".
+Definition ___builtin_debug : ident := $"__builtin_debug".
+Definition ___builtin_expect : ident := $"__builtin_expect".
+Definition ___builtin_fabs : ident := $"__builtin_fabs".
+Definition ___builtin_fabsf : ident := $"__builtin_fabsf".
+Definition ___builtin_fmadd : ident := $"__builtin_fmadd".
+Definition ___builtin_fmax : ident := $"__builtin_fmax".
+Definition ___builtin_fmin : ident := $"__builtin_fmin".
+Definition ___builtin_fmsub : ident := $"__builtin_fmsub".
+Definition ___builtin_fnmadd : ident := $"__builtin_fnmadd".
+Definition ___builtin_fnmsub : ident := $"__builtin_fnmsub".
+Definition ___builtin_fsqrt : ident := $"__builtin_fsqrt".
+Definition ___builtin_membar : ident := $"__builtin_membar".
+Definition ___builtin_memcpy_aligned : ident := $"__builtin_memcpy_aligned".
+Definition ___builtin_read16_reversed : ident := $"__builtin_read16_reversed".
+Definition ___builtin_read32_reversed : ident := $"__builtin_read32_reversed".
+Definition ___builtin_sel : ident := $"__builtin_sel".
+Definition ___builtin_sqrt : ident := $"__builtin_sqrt".
+Definition ___builtin_unreachable : ident := $"__builtin_unreachable".
+Definition ___builtin_va_arg : ident := $"__builtin_va_arg".
+Definition ___builtin_va_copy : ident := $"__builtin_va_copy".
+Definition ___builtin_va_end : ident := $"__builtin_va_end".
+Definition ___builtin_va_start : ident := $"__builtin_va_start".
+Definition ___builtin_write16_reversed : ident := $"__builtin_write16_reversed".
+Definition ___builtin_write32_reversed : ident := $"__builtin_write32_reversed".
+Definition ___compcert_i64_dtos : ident := $"__compcert_i64_dtos".
+Definition ___compcert_i64_dtou : ident := $"__compcert_i64_dtou".
+Definition ___compcert_i64_sar : ident := $"__compcert_i64_sar".
+Definition ___compcert_i64_sdiv : ident := $"__compcert_i64_sdiv".
+Definition ___compcert_i64_shl : ident := $"__compcert_i64_shl".
+Definition ___compcert_i64_shr : ident := $"__compcert_i64_shr".
+Definition ___compcert_i64_smod : ident := $"__compcert_i64_smod".
+Definition ___compcert_i64_smulh : ident := $"__compcert_i64_smulh".
+Definition ___compcert_i64_stod : ident := $"__compcert_i64_stod".
+Definition ___compcert_i64_stof : ident := $"__compcert_i64_stof".
+Definition ___compcert_i64_udiv : ident := $"__compcert_i64_udiv".
+Definition ___compcert_i64_umod : ident := $"__compcert_i64_umod".
+Definition ___compcert_i64_umulh : ident := $"__compcert_i64_umulh".
+Definition ___compcert_i64_utod : ident := $"__compcert_i64_utod".
+Definition ___compcert_i64_utof : ident := $"__compcert_i64_utof".
+Definition ___compcert_va_composite : ident := $"__compcert_va_composite".
+Definition ___compcert_va_float64 : ident := $"__compcert_va_float64".
+Definition ___compcert_va_int32 : ident := $"__compcert_va_int32".
+Definition ___compcert_va_int64 : ident := $"__compcert_va_int64".
+Definition _a : ident := $"a".
+Definition _b : ident := $"b".
+Definition _c : ident := $"c".
+Definition _cross32 : ident := $"cross32".
+Definition _cur : ident := $"cur".
+Definition _f : ident := $"f".
+Definition _f2i : ident := $"f2i".
+Definition _f_or_i : ident := $"f_or_i".
+Definition _i : ident := $"i".
+Definition _main : ident := $"main".
+Definition _newlo : ident := $"newlo".
+Definition _old : ident := $"old".
+Definition _ptr_only : ident := $"ptr_only".
+Definition _ptr_ptr_mix : ident := $"ptr_ptr_mix".
+Definition _ptr_r32_after_w32 : ident := $"ptr_r32_after_w32".
+Definition _ptr_r64_after_w32 : ident := $"ptr_r64_after_w32".
+Definition _ptr_r64_after_w64 : ident := $"ptr_r64_after_w64".
+Definition _r32_r64_w64 : ident := $"r32_r64_w64".
+Definition _res : ident := $"res".
+Definition _rw32 : ident := $"rw32".
+Definition _rw64 : ident := $"rw64".
+Definition _s : ident := $"s".
+Definition _seed : ident := $"seed".
+Definition _twin32 : ident := $"twin32".
+Definition _u : ident := $"u".
+Definition _v32 : ident := $"v32".
+Definition _v64 : ident := $"v64".
+Definition _w : ident := $"w".
+Definition _w0_r32 : ident := $"w0_r32".
+Definition _w64_r32 : ident := $"w64_r32".
+Definition _w64_w32_r64 : ident := $"w64_w32_r64".
+Definition _x : ident := $"x".
+Definition _t'1 : ident := 128%positive.
+
+Definition f_rw32 := {|
+  fn_return := tuint;
+  fn_callconv := cc_default;
+  fn_params := ((_s, (tptr (Tunion _seed noattr))) :: (_x, tuint) :: nil);
+  fn_vars := nil;
+  fn_temps := ((_t'1, tuint) :: nil);
+  fn_body :=
+(Ssequence
+  (Sassign
+    (Efield
+      (Ederef (Etempvar _s (tptr (Tunion _seed noattr)))
+        (Tunion _seed noattr)) _v32 tuint) (Etempvar _x tuint))
+  (Ssequence
+    (Sset _t'1
+      (Efield
+        (Ederef (Etempvar _s (tptr (Tunion _seed noattr)))
+          (Tunion _seed noattr)) _v32 tuint))
+    (Sreturn (Some (Etempvar _t'1 tuint)))))
+|}.
+
+Definition f_rw64 := {|
+  fn_return := tulong;
+  fn_callconv := cc_default;
+  fn_params := ((_s, (tptr (Tunion _seed noattr))) :: (_c, tulong) :: nil);
+  fn_vars := nil;
+  fn_temps := ((_t'1, tulong) :: nil);
+  fn_body :=
+(Ssequence
+  (Sassign
+    (Efield
+      (Ederef (Etempvar _s (tptr (Tunion _seed noattr)))
+        (Tunion _seed noattr)) _v64 tulong) (Etempvar _c tulong))
+  (Ssequence
+    (Sset _t'1
+      (Efield
+        (Ederef (Etempvar _s (tptr (Tunion _seed noattr)))
+          (Tunion _seed noattr)) _v64 tulong))
+    (Sreturn (Some (Etempvar _t'1 tulong)))))
+|}.
+
+Definition f_w64_r32 := {|
+  fn_return := tuint;
+  fn_callconv := cc_default;
+  fn_params := ((_s, (tptr (Tunion _seed noattr))) :: (_c, tulong) :: nil);
+  fn_vars := nil;
+  fn_temps := ((_t'1, tuint) :: nil);
+  fn_body :=
+(Ssequence
+  (Sassign
+    (Efield
+      (Ederef (Etempvar _s (tptr (Tunion _seed noattr)))
+        (Tunion _seed noattr)) _v64 tulong) (Etempvar _c tulong))
+  (Ssequence
+    (Sset _t'1
+      (Efield
+        (Ederef (Etempvar _s (tptr (Tunion _seed noattr)))
+          (Tunion _seed noattr)) _v32 tuint))
+    (Sreturn (Some (Etempvar _t'1 tuint)))))
+|}.
+
+Definition f_w64_w32_r64 := {|
+  fn_return := tulong;
+  fn_callconv := cc_default;
+  fn_params := ((_s, (tptr (Tunion _seed noattr))) :: (_c, tulong) ::
+                (_x, tuint) :: nil);
+  fn_vars := nil;
+  fn_temps := ((_t'1, tulong) :: nil);
+  fn_body :=
+(Ssequence
+  (Sassign
+    (Efield
+      (Ederef (Etempvar _s (tptr (Tunion _seed noattr)))
+        (Tunion _seed noattr)) _v64 tulong) (Etempvar _c tulong))
+  (Ssequence
+    (Sassign
+      (Efield
+        (Ederef (Etempvar _s (tptr (Tunion _seed noattr)))
+          (Tunion _seed noattr)) _v32 tuint) (Etempvar _x tuint))
+    (Ssequence
+      (Sset _t'1
+        (Efield
+          (Ederef (Etempvar _s (tptr (Tunion _seed noattr)))
+            (Tunion _seed noattr)) _v64 tulong))
+      (Sreturn (Some (Etempvar _t'1 tulong))))))
+|}.
+
+Definition f_ptr_r64_after_w64 := {|
+  fn_return := tulong;
+  fn_callconv := cc_default;
+  fn_params := ((_s, (tptr (Tunion _seed noattr))) :: (_c, tulong) :: nil);
+  fn_vars := nil;
+  fn_temps := ((_t'1, tulong) :: nil);
+  fn_body :=
+(Ssequence
+  (Sassign
+    (Efield
+      (Ederef (Etempvar _s (tptr (Tunion _seed noattr)))
+        (Tunion _seed noattr)) _v64 tulong) (Etempvar _c tulong))
+  (Ssequence
+    (Sset _t'1
+      (Ederef
+        (Ecast (Etempvar _s (tptr (Tunion _seed noattr))) (tptr tulong))
+        tulong))
+    (Sreturn (Some (Etempvar _t'1 tulong)))))
+|}.
+
+Definition f_ptr_r32_after_w32 := {|
+  fn_return := tuint;
+  fn_callconv := cc_default;
+  fn_params := ((_s, (tptr (Tunion _seed noattr))) :: (_x, tuint) :: nil);
+  fn_vars := nil;
+  fn_temps := ((_t'1, tuint) :: nil);
+  fn_body :=
+(Ssequence
+  (Sassign
+    (Efield
+      (Ederef (Etempvar _s (tptr (Tunion _seed noattr)))
+        (Tunion _seed noattr)) _v32 tuint) (Etempvar _x tuint))
+  (Ssequence
+    (Sset _t'1
+      (Ederef (Ecast (Etempvar _s (tptr (Tunion _seed noattr))) (tptr tuint))
+        tuint))
+    (Sreturn (Some (Etempvar _t'1 tuint)))))
+|}.
+
+Definition f_ptr_r64_after_w32 := {|
+  fn_return := tulong;
+  fn_callconv := cc_default;
+  fn_params := ((_s, (tptr (Tunion _seed noattr))) :: (_x, tuint) :: nil);
+  fn_vars := nil;
+  fn_temps := ((_t'1, tulong) :: nil);
+  fn_body :=
+(Ssequence
+  (Sassign
+    (Efield
+      (Ederef (Etempvar _s (tptr (Tunion _seed noattr)))
+        (Tunion _seed noattr)) _v32 tuint) (Etempvar _x tuint))
+  (Ssequence
+    (Sset _t'1
+      (Ederef
+        (Ecast (Etempvar _s (tptr (Tunion _seed noattr))) (tptr tulong))
+        tulong))
+    (Sreturn (Some (Etempvar _t'1 tulong)))))
+|}.
+
+Definition f_ptr_ptr_mix := {|
+  fn_return := tulong;
+  fn_callconv := cc_default;
+  fn_params := ((_w, (tptr tulong)) :: (_x, tuint) :: nil);
+  fn_vars := nil;
+  fn_temps := ((_t'1, tulong) :: nil);
+  fn_body :=
+(Ssequence
+  (Sassign (Ederef (Ecast (Etempvar _w (tptr tulong)) (tptr tuint)) tuint)
+    (Etempvar _x tuint))
+  (Ssequence
+    (Sset _t'1 (Ederef (Etempvar _w (tptr tulong)) tulong))
+    (Sreturn (Some (Etempvar _t'1 tulong)))))
+|}.
+
+Definition f_ptr_only := {|
+  fn_return := tulong;
+  fn_callconv := cc_default;
+  fn_params := ((_w, (tptr tulong)) :: (_x, tuint) :: nil);
+  fn_vars := nil;
+  fn_temps := ((_t'1, tulong) :: nil);
+  fn_body :=
+(Ssequence
+  (Sassign (Ederef (Etempvar _w (tptr tulong)) tulong) (Etempvar _x tuint))
+  (Ssequence
+    (Sset _t'1 (Ederef (Etempvar _w (tptr tulong)) tulong))
+    (Sreturn (Some (Etempvar _t'1 tulong)))))
+|}.
+
+Definition f_w0_r32 := {|
+  fn_return := tuint;
+  fn_callconv := cc_default;
+  fn_params := ((_s, (tptr (Tunion _seed noattr))) :: nil);
+  fn_vars := nil;
+  fn_temps := ((_t'1, tuint) :: nil);
+  fn_body :=
+(Ssequence
+  (Sassign
+    (Efield
+      (Ederef (Etempvar _s (tptr (Tunion _seed noattr)))
+        (Tunion _seed noattr)) _v64 tulong) (Econst_int (Int.repr 0) tint))
+  (Ssequence
+    (Sset _t'1
+      (Efield
+        (Ederef (Etempvar _s (tptr (Tunion _seed noattr)))
+          (Tunion _seed noattr)) _v32 tuint))
+    (Sreturn (Some (Etempvar _t'1 tuint)))))
+|}.
+
+Definition f_r32_r64_w64 := {|
+  fn_return := tulong;
+  fn_callconv := cc_default;
+  fn_params := ((_s, (tptr (Tunion _seed noattr))) :: (_newlo, tuint) :: nil);
+  fn_vars := nil;
+  fn_temps := ((_old, tuint) :: (_cur, tulong) :: (_res, tulong) :: nil);
+  fn_body :=
+(Ssequence
+  (Sset _old
+    (Efield
+      (Ederef (Etempvar _s (tptr (Tunion _seed noattr)))
+        (Tunion _seed noattr)) _v32 tuint))
+  (Ssequence
+    (Sset _cur
+      (Efield
+        (Ederef (Etempvar _s (tptr (Tunion _seed noattr)))
+          (Tunion _seed noattr)) _v64 tulong))
+    (Ssequence
+      (Sset _res
+        (Ebinop Oadd
+          (Ebinop Osub (Etempvar _cur tulong) (Etempvar _old tuint) tulong)
+          (Etempvar _newlo tuint) tulong))
+      (Ssequence
+        (Sassign
+          (Efield
+            (Ederef (Etempvar _s (tptr (Tunion _seed noattr)))
+              (Tunion _seed noattr)) _v64 tulong) (Etempvar _res tulong))
+        (Sreturn (Some (Etempvar _res tulong)))))))
+|}.
+
+Definition f_cross32 := {|
+  fn_return := tuint;
+  fn_callconv := cc_default;
+  fn_params := ((_u, (tptr (Tunion _twin32 noattr))) :: (_x, tuint) :: nil);
+  fn_vars := nil;
+  fn_temps := ((_t'1, tuint) :: nil);
+  fn_body :=
+(Ssequence
+  (Sassign
+    (Efield
+      (Ederef (Etempvar _u (tptr (Tunion _twin32 noattr)))
+        (Tunion _twin32 noattr)) _a tuint) (Etempvar _x tuint))
+  (Ssequence
+    (Sset _t'1
+      (Efield
+        (Ederef (Etempvar _u (tptr (Tunion _twin32 noattr)))
+          (Tunion _twin32 noattr)) _b tuint))
+    (Sreturn (Some (Etempvar _t'1 tuint)))))
+|}.
+
+Definition f_f2i := {|
+  fn_return := tuint;
+  fn_callconv := cc_default;
+  fn_params := ((_x, tfloat) :: nil);
+  fn_vars := ((_u, (Tunion _f_or_i noattr)) :: nil);
+  fn_temps := ((_t'1, tuint) :: nil);
+  fn_body :=
+(Ssequence
+  (Sassign (Efield (Evar _u (Tunion _f_or_i noattr)) _f tfloat)
+    (Etempvar _x tfloat))
+  (Ssequence
+    (Sset _t'1 (Efield (Evar _u (Tunion _f_or_i noattr)) _i tuint))
+    (Sreturn (Some (Etempvar _t'1 tuint)))))
+|}.
+
+Definition composites : list composite_definition :=
+(Composite _seed Union
+   (Member_plain _v32 tuint :: Member_plain _v64 tulong :: nil)
+   noattr ::
+ Composite _twin32 Union
+   (Member_plain _a tuint :: Member_plain _b tuint :: nil)
+   noattr ::
+ Composite _f_or_i Union
+   (Member_plain _f tfloat :: Member_plain _i tuint :: nil)
+   noattr :: nil).
+
+Definition global_definitions : list (ident * globdef fundef type) :=
+((___compcert_va_int32,
+   Gfun(External (EF_runtime "__compcert_va_int32"
+                   (mksignature (AST.Xptr :: nil) AST.Xint cc_default))
+     ((tptr tvoid) :: nil) tuint cc_default)) ::
+ (___compcert_va_int64,
+   Gfun(External (EF_runtime "__compcert_va_int64"
+                   (mksignature (AST.Xptr :: nil) AST.Xlong cc_default))
+     ((tptr tvoid) :: nil) tulong cc_default)) ::
+ (___compcert_va_float64,
+   Gfun(External (EF_runtime "__compcert_va_float64"
+                   (mksignature (AST.Xptr :: nil) AST.Xfloat cc_default))
+     ((tptr tvoid) :: nil) tdouble cc_default)) ::
+ (___compcert_va_composite,
+   Gfun(External (EF_runtime "__compcert_va_composite"
+                   (mksignature (AST.Xptr :: AST.Xlong :: nil) AST.Xptr
+                     cc_default)) ((tptr tvoid) :: tulong :: nil)
+     (tptr tvoid) cc_default)) ::
+ (___compcert_i64_dtos,
+   Gfun(External (EF_runtime "__compcert_i64_dtos"
+                   (mksignature (AST.Xfloat :: nil) AST.Xlong cc_default))
+     (tdouble :: nil) tlong cc_default)) ::
+ (___compcert_i64_dtou,
+   Gfun(External (EF_runtime "__compcert_i64_dtou"
+                   (mksignature (AST.Xfloat :: nil) AST.Xlong cc_default))
+     (tdouble :: nil) tulong cc_default)) ::
+ (___compcert_i64_stod,
+   Gfun(External (EF_runtime "__compcert_i64_stod"
+                   (mksignature (AST.Xlong :: nil) AST.Xfloat cc_default))
+     (tlong :: nil) tdouble cc_default)) ::
+ (___compcert_i64_utod,
+   Gfun(External (EF_runtime "__compcert_i64_utod"
+                   (mksignature (AST.Xlong :: nil) AST.Xfloat cc_default))
+     (tulong :: nil) tdouble cc_default)) ::
+ (___compcert_i64_stof,
+   Gfun(External (EF_runtime "__compcert_i64_stof"
+                   (mksignature (AST.Xlong :: nil) AST.Xsingle cc_default))
+     (tlong :: nil) tfloat cc_default)) ::
+ (___compcert_i64_utof,
+   Gfun(External (EF_runtime "__compcert_i64_utof"
+                   (mksignature (AST.Xlong :: nil) AST.Xsingle cc_default))
+     (tulong :: nil) tfloat cc_default)) ::
+ (___compcert_i64_sdiv,
+   Gfun(External (EF_runtime "__compcert_i64_sdiv"
+                   (mksignature (AST.Xlong :: AST.Xlong :: nil) AST.Xlong
+                     cc_default)) (tlong :: tlong :: nil) tlong cc_default)) ::
+ (___compcert_i64_udiv,
+   Gfun(External (EF_runtime "__compcert_i64_udiv"
+                   (mksignature (AST.Xlong :: AST.Xlong :: nil) AST.Xlong
+                     cc_default)) (tulong :: tulong :: nil) tulong
+     cc_default)) ::
+ (___compcert_i64_smod,
+   Gfun(External (EF_runtime "__compcert_i64_smod"
+                   (mksignature (AST.Xlong :: AST.Xlong :: nil) AST.Xlong
+                     cc_default)) (tlong :: tlong :: nil) tlong cc_default)) ::
+ (___compcert_i64_umod,
+   Gfun(External (EF_runtime "__compcert_i64_umod"
+                   (mksignature (AST.Xlong :: AST.Xlong :: nil) AST.Xlong
+                     cc_default)) (tulong :: tulong :: nil) tulong
+     cc_default)) ::
+ (___compcert_i64_shl,
+   Gfun(External (EF_runtime "__compcert_i64_shl"
+                   (mksignature (AST.Xlong :: AST.Xint :: nil) AST.Xlong
+                     cc_default)) (tlong :: tint :: nil) tlong cc_default)) ::
+ (___compcert_i64_shr,
+   Gfun(External (EF_runtime "__compcert_i64_shr"
+                   (mksignature (AST.Xlong :: AST.Xint :: nil) AST.Xlong
+                     cc_default)) (tulong :: tint :: nil) tulong cc_default)) ::
+ (___compcert_i64_sar,
+   Gfun(External (EF_runtime "__compcert_i64_sar"
+                   (mksignature (AST.Xlong :: AST.Xint :: nil) AST.Xlong
+                     cc_default)) (tlong :: tint :: nil) tlong cc_default)) ::
+ (___compcert_i64_smulh,
+   Gfun(External (EF_runtime "__compcert_i64_smulh"
+                   (mksignature (AST.Xlong :: AST.Xlong :: nil) AST.Xlong
+                     cc_default)) (tlong :: tlong :: nil) tlong cc_default)) ::
+ (___compcert_i64_umulh,
+   Gfun(External (EF_runtime "__compcert_i64_umulh"
+                   (mksignature (AST.Xlong :: AST.Xlong :: nil) AST.Xlong
+                     cc_default)) (tulong :: tulong :: nil) tulong
+     cc_default)) ::
+ (___builtin_ais_annot,
+   Gfun(External (EF_builtin "__builtin_ais_annot"
+                   (mksignature (AST.Xptr :: nil) AST.Xvoid
+                     {|cc_vararg:=(Some 1); cc_unproto:=false; cc_structret:=false|}))
+     ((tptr tschar) :: nil) tvoid
+     {|cc_vararg:=(Some 1); cc_unproto:=false; cc_structret:=false|})) ::
+ (___builtin_bswap64,
+   Gfun(External (EF_builtin "__builtin_bswap64"
+                   (mksignature (AST.Xlong :: nil) AST.Xlong cc_default))
+     (tulong :: nil) tulong cc_default)) ::
+ (___builtin_bswap,
+   Gfun(External (EF_builtin "__builtin_bswap"
+                   (mksignature (AST.Xint :: nil) AST.Xint cc_default))
+     (tuint :: nil) tuint cc_default)) ::
+ (___builtin_bswap32,
+   Gfun(External (EF_builtin "__builtin_bswap32"
+                   (mksignature (AST.Xint :: nil) AST.Xint cc_default))
+     (tuint :: nil) tuint cc_default)) ::
+ (___builtin_bswap16,
+   Gfun(External (EF_builtin "__builtin_bswap16"
+                   (mksignature (AST.Xint16unsigned :: nil)
+                     AST.Xint16unsigned cc_default)) (tushort :: nil) tushort
+     cc_default)) ::
+ (___builtin_clz,
+   Gfun(External (EF_builtin "__builtin_clz"
+                   (mksignature (AST.Xint :: nil) AST.Xint cc_default))
+     (tuint :: nil) tint cc_default)) ::
+ (___builtin_clzl,
+   Gfun(External (EF_builtin "__builtin_clzl"
+                   (mksignature (AST.Xlong :: nil) AST.Xint cc_default))
+     (tulong :: nil) tint cc_default)) ::
+ (___builtin_clzll,
+   Gfun(External (EF_builtin "__builtin_clzll"
+                   (mksignature (AST.Xlong :: nil) AST.Xint cc_default))
+     (tulong :: nil) tint cc_default)) ::
+ (___builtin_ctz,
+   Gfun(External (EF_builtin "__builtin_ctz"
+                   (mksignature (AST.Xint :: nil) AST.Xint cc_default))
+     (tuint :: nil) tint cc_default)) ::
+ (___builtin_ctzl,
+   Gfun(External (EF_builtin "__builtin_ctzl"
+                   (mksignature (AST.Xlong :: nil) AST.Xint cc_default))
+     (tulong :: nil) tint cc_default)) ::
+ (___builtin_ctzll,
+   Gfun(External (EF_builtin "__builtin_ctzll"
+                   (mksignature (AST.Xlong :: nil) AST.Xint cc_default))
+     (tulong :: nil) tint cc_default)) ::
+ (___builtin_fabs,
+   Gfun(External (EF_builtin "__builtin_fabs"
+                   (mksignature (AST.Xfloat :: nil) AST.Xfloat cc_default))
+     (tdouble :: nil) tdouble cc_default)) ::
+ (___builtin_fabsf,
+   Gfun(External (EF_builtin "__builtin_fabsf"
+                   (mksignature (AST.Xsingle :: nil) AST.Xsingle cc_default))
+     (tfloat :: nil) tfloat cc_default)) ::
+ (___builtin_fsqrt,
+   Gfun(External (EF_builtin "__builtin_fsqrt"
+                   (mksignature (AST.Xfloat :: nil) AST.Xfloat cc_default))
+     (tdouble :: nil) tdouble cc_default)) ::
+ (___builtin_sqrt,
+   Gfun(External (EF_builtin "__builtin_sqrt"
+                   (mksignature (AST.Xfloat :: nil) AST.Xfloat cc_default))
+     (tdouble :: nil) tdouble cc_default)) ::
+ (___builtin_memcpy_aligned,
+   Gfun(External (EF_builtin "__builtin_memcpy_aligned"
+                   (mksignature
+                     (AST.Xptr :: AST.Xptr :: AST.Xlong :: AST.Xlong :: nil)
+                     AST.Xvoid cc_default))
+     ((tptr tvoid) :: (tptr tvoid) :: tulong :: tulong :: nil) tvoid
+     cc_default)) ::
+ (___builtin_sel,
+   Gfun(External (EF_builtin "__builtin_sel"
+                   (mksignature (AST.Xbool :: nil) AST.Xvoid
+                     {|cc_vararg:=(Some 1); cc_unproto:=false; cc_structret:=false|}))
+     (tbool :: nil) tvoid
+     {|cc_vararg:=(Some 1); cc_unproto:=false; cc_structret:=false|})) ::
+ (___builtin_annot,
+   Gfun(External (EF_builtin "__builtin_annot"
+                   (mksignature (AST.Xptr :: nil) AST.Xvoid
+                     {|cc_vararg:=(Some 1); cc_unproto:=false; cc_structret:=false|}))
+     ((tptr tschar) :: nil) tvoid
+     {|cc_vararg:=(Some 1); cc_unproto:=false; cc_structret:=false|})) ::
+ (___builtin_annot_intval,
+   Gfun(External (EF_builtin "__builtin_annot_intval"
+                   (mksignature (AST.Xptr :: AST.Xint :: nil) AST.Xint
+                     cc_default)) ((tptr tschar) :: tint :: nil) tint
+     cc_default)) ::
+ (___builtin_membar,
+   Gfun(External (EF_builtin "__builtin_membar"
+                   (mksignature nil AST.Xvoid cc_default)) nil tvoid
+     cc_default)) ::
+ (___builtin_va_start,
+   Gfun(External (EF_builtin "__builtin_va_start"
+                   (mksignature (AST.Xptr :: nil) AST.Xvoid cc_default))
+     ((tptr tvoid) :: nil) tvoid cc_default)) ::
+ (___builtin_va_arg,
+   Gfun(External (EF_builtin "__builtin_va_arg"
+                   (mksignature (AST.Xptr :: AST.Xint :: nil) AST.Xvoid
+                     cc_default)) ((tptr tvoid) :: tuint :: nil) tvoid
+     cc_default)) ::
+ (___builtin_va_copy,
+   Gfun(External (EF_builtin "__builtin_va_copy"
+                   (mksignature (AST.Xptr :: AST.Xptr :: nil) AST.Xvoid
+                     cc_default)) ((tptr tvoid) :: (tptr tvoid) :: nil) tvoid
+     cc_default)) ::
+ (___builtin_va_end,
+   Gfun(External (EF_builtin "__builtin_va_end"
+                   (mksignature (AST.Xptr :: nil) AST.Xvoid cc_default))
+     ((tptr tvoid) :: nil) tvoid cc_default)) ::
+ (___builtin_unreachable,
+   Gfun(External (EF_builtin "__builtin_unreachable"
+                   (mksignature nil AST.Xvoid cc_default)) nil tvoid
+     cc_default)) ::
+ (___builtin_expect,
+   Gfun(External (EF_builtin "__builtin_expect"
+                   (mksignature (AST.Xlong :: AST.Xlong :: nil) AST.Xlong
+                     cc_default)) (tlong :: tlong :: nil) tlong cc_default)) ::
+ (___builtin_fmax,
+   Gfun(External (EF_builtin "__builtin_fmax"
+                   (mksignature (AST.Xfloat :: AST.Xfloat :: nil) AST.Xfloat
+                     cc_default)) (tdouble :: tdouble :: nil) tdouble
+     cc_default)) ::
+ (___builtin_fmin,
+   Gfun(External (EF_builtin "__builtin_fmin"
+                   (mksignature (AST.Xfloat :: AST.Xfloat :: nil) AST.Xfloat
+                     cc_default)) (tdouble :: tdouble :: nil) tdouble
+     cc_default)) ::
+ (___builtin_fmadd,
+   Gfun(External (EF_builtin "__builtin_fmadd"
+                   (mksignature
+                     (AST.Xfloat :: AST.Xfloat :: AST.Xfloat :: nil)
+                     AST.Xfloat cc_default))
+     (tdouble :: tdouble :: tdouble :: nil) tdouble cc_default)) ::
+ (___builtin_fmsub,
+   Gfun(External (EF_builtin "__builtin_fmsub"
+                   (mksignature
+                     (AST.Xfloat :: AST.Xfloat :: AST.Xfloat :: nil)
+                     AST.Xfloat cc_default))
+     (tdouble :: tdouble :: tdouble :: nil) tdouble cc_default)) ::
+ (___builtin_fnmadd,
+   Gfun(External (EF_builtin "__builtin_fnmadd"
+                   (mksignature
+                     (AST.Xfloat :: AST.Xfloat :: AST.Xfloat :: nil)
+                     AST.Xfloat cc_default))
+     (tdouble :: tdouble :: tdouble :: nil) tdouble cc_default)) ::
+ (___builtin_fnmsub,
+   Gfun(External (EF_builtin "__builtin_fnmsub"
+                   (mksignature
+                     (AST.Xfloat :: AST.Xfloat :: AST.Xfloat :: nil)
+                     AST.Xfloat cc_default))
+     (tdouble :: tdouble :: tdouble :: nil) tdouble cc_default)) ::
+ (___builtin_read16_reversed,
+   Gfun(External (EF_builtin "__builtin_read16_reversed"
+                   (mksignature (AST.Xptr :: nil) AST.Xint16unsigned
+                     cc_default)) ((tptr tushort) :: nil) tushort
+     cc_default)) ::
+ (___builtin_read32_reversed,
+   Gfun(External (EF_builtin "__builtin_read32_reversed"
+                   (mksignature (AST.Xptr :: nil) AST.Xint cc_default))
+     ((tptr tuint) :: nil) tuint cc_default)) ::
+ (___builtin_write16_reversed,
+   Gfun(External (EF_builtin "__builtin_write16_reversed"
+                   (mksignature (AST.Xptr :: AST.Xint16unsigned :: nil)
+                     AST.Xvoid cc_default))
+     ((tptr tushort) :: tushort :: nil) tvoid cc_default)) ::
+ (___builtin_write32_reversed,
+   Gfun(External (EF_builtin "__builtin_write32_reversed"
+                   (mksignature (AST.Xptr :: AST.Xint :: nil) AST.Xvoid
+                     cc_default)) ((tptr tuint) :: tuint :: nil) tvoid
+     cc_default)) ::
+ (___builtin_debug,
+   Gfun(External (EF_external "__builtin_debug"
+                   (mksignature (AST.Xint :: nil) AST.Xvoid
+                     {|cc_vararg:=(Some 1); cc_unproto:=false; cc_structret:=false|}))
+     (tint :: nil) tvoid
+     {|cc_vararg:=(Some 1); cc_unproto:=false; cc_structret:=false|})) ::
+ (_rw32, Gfun(Internal f_rw32)) :: (_rw64, Gfun(Internal f_rw64)) ::
+ (_w64_r32, Gfun(Internal f_w64_r32)) ::
+ (_w64_w32_r64, Gfun(Internal f_w64_w32_r64)) ::
+ (_ptr_r64_after_w64, Gfun(Internal f_ptr_r64_after_w64)) ::
+ (_ptr_r32_after_w32, Gfun(Internal f_ptr_r32_after_w32)) ::
+ (_ptr_r64_after_w32, Gfun(Internal f_ptr_r64_after_w32)) ::
+ (_ptr_ptr_mix, Gfun(Internal f_ptr_ptr_mix)) ::
+ (_ptr_only, Gfun(Internal f_ptr_only)) ::
+ (_w0_r32, Gfun(Internal f_w0_r32)) ::
+ (_r32_r64_w64, Gfun(Internal f_r32_r64_w64)) ::
+ (_cross32, Gfun(Internal f_cross32)) :: (_f2i, Gfun(Internal f_f2i)) :: nil).
+
+Definition public_idents : list ident :=
+(_f2i :: _cross32 :: _r32_r64_w64 :: _w0_r32 :: _ptr_only :: _ptr_ptr_mix ::
+ _ptr_r64_after_w32 :: _ptr_r32_after_w32 :: _ptr_r64_after_w64 ::
+ _w64_w32_r64 :: _w64_r32 :: _rw64 :: _rw32 :: ___builtin_debug ::
+ ___builtin_write32_reversed :: ___builtin_write16_reversed ::
+ ___builtin_read32_reversed :: ___builtin_read16_reversed ::
+ ___builtin_fnmsub :: ___builtin_fnmadd :: ___builtin_fmsub ::
+ ___builtin_fmadd :: ___builtin_fmin :: ___builtin_fmax ::
+ ___builtin_expect :: ___builtin_unreachable :: ___builtin_va_end ::
+ ___builtin_va_copy :: ___builtin_va_arg :: ___builtin_va_start ::
+ ___builtin_membar :: ___builtin_annot_intval :: ___builtin_annot ::
+ ___builtin_sel :: ___builtin_memcpy_aligned :: ___builtin_sqrt ::
+ ___builtin_fsqrt :: ___builtin_fabsf :: ___builtin_fabs ::
+ ___builtin_ctzll :: ___builtin_ctzl :: ___builtin_ctz :: ___builtin_clzll ::
+ ___builtin_clzl :: ___builtin_clz :: ___builtin_bswap16 ::
+ ___builtin_bswap32 :: ___builtin_bswap :: ___builtin_bswap64 ::
+ ___builtin_ais_annot :: ___compcert_i64_umulh :: ___compcert_i64_smulh ::
+ ___compcert_i64_sar :: ___compcert_i64_shr :: ___compcert_i64_shl ::
+ ___compcert_i64_umod :: ___compcert_i64_smod :: ___compcert_i64_udiv ::
+ ___compcert_i64_sdiv :: ___compcert_i64_utof :: ___compcert_i64_stof ::
+ ___compcert_i64_utod :: ___compcert_i64_stod :: ___compcert_i64_dtou ::
+ ___compcert_i64_dtos :: ___compcert_va_composite ::
+ ___compcert_va_float64 :: ___compcert_va_int64 :: ___compcert_va_int32 ::
+ nil).
+
+Definition prog : Clight.program :=
+  mkprogram composites global_definitions public_idents _main Logic.I.
+
