fusion/tests/union_exact_seed_spec.v
@@ -1,0 +1,27 @@
+Require Import VST.floyd.proofauto.
+Require Import VST.floyd.library.
+Require Import seed_union_rw bridges union_exact_view union_exact_seed_interface union_exact_seed_support.
+
+Module SeedSpec (Import Layout : SEED_LAYOUT).
+Include SeedSupport Layout.
+Local Existing Instance CompSpecs.
+Local Open Scope Z.
+Local Open Scope logic.
+
+Definition tseed_exact := Tunion _seed noattr.
+Definition seed_v64_exact (sh : share) (x : int64) (p : val) : mpred :=
+  exact_seed_v64 sh x p.
+
+Definition w64_r32_exact_spec : ident * funspec :=
+  DECLARE _w64_r32
+  WITH c0 : int64, x : int64, s : val
+  PRE [tptr tseed_exact, tulong]
+    PROP ()
+    PARAMS (s; Vlong x)
+    SEP (data_at Ews tseed_exact (seed_value c0) s)
+  POST [tuint]
+    PROP ()
+    RETURN (Vint (Int64.loword x))
+    SEP (seed_v64_exact Ews x s).
+
+End SeedSpec.
