fusion/tests/union_exact_seed_support.v
@@ -1,0 +1,196 @@
+(* Proved seed-union assertions and load adapters. *)
+
+Require Import VST.floyd.proofauto.
+Require Import VST.floyd.library.
+Require Import seed_union_rw union_exact_seed_interface.
+Require Import union_exact_view.
+
+Module SeedSupport (Import Layout : SEED_LAYOUT).
+Local Existing Instance CompSpecs.
+
+Local Open Scope logic.
+
+Definition exact_seed_type := Tunion _seed noattr.
+
+Definition exact_seed_v64 (sh : share) (x : int64) (p : val) : mpred :=
+  !! field_compatible exact_seed_type [] p &&
+  exact_mapsto sh Mint64 (Vlong x) p.
+
+Definition seed_data_v64 (sh : share) (x : int64) (p : val) : mpred :=
+  data_at sh exact_seed_type (seed_value x) p.
+
+Lemma exact_seed_v64_isptr : forall sh x p,
+  exact_seed_v64 sh x p |-- !! isptr p.
+Proof.
+  intros. unfold exact_seed_v64.
+  apply andp_left1. apply prop_derives.
+  intros [Hptr _]. exact Hptr.
+Qed.
+
+Definition seed_store_v64_lvalue : expr :=
+    (Efield
+      (Ederef (Etempvar _s (tptr exact_seed_type)) exact_seed_type)
+      _v64 tulong).
+
+Definition seed_store_v64_value : expr := Etempvar _c tulong.
+
+Definition seed_store_v64_statement : statement :=
+  Sassign seed_store_v64_lvalue seed_store_v64_value.
+
+Definition seed_load_v32_expr : expr :=
+    (Efield
+      (Ederef (Etempvar _s (tptr exact_seed_type)) exact_seed_type)
+      _v32 tuint).
+
+Definition seed_load_v32_statement : statement :=
+  Sset _t'1 seed_load_v32_expr.
+
+Lemma seed_store_v64_address : forall Delta c0 x s,
+  ENTAIL Delta,
+    PROP () LOCAL (temp _s s; temp _c (Vlong x))
+    SEP (seed_data_v64 Ews c0 s) |--
+    local (fun rho => s = eval_lvalue seed_store_v64_lvalue rho).
+Proof.
+  intros. unfold seed_store_v64_lvalue, seed_data_v64.
+  rewrite data_at_isptr.
+  apply andp_left2. intro rho.
+  unfold PROPx, LOCALx, SEPx. simpl.
+  unfold local, lift1. unfold_lift. simpl.
+  constructor. intros w H.
+  destruct H as [_ Hrest]. simpl in Hrest |- *.
+  destruct Hrest as [Hlocals Hsep].
+  destruct Hlocals as [[Hs _] _].
+  destruct Hsep as [w1 [w2 [_ [Hdata _]]]].
+  destruct Hdata as [Hptr _].
+  rewrite <- Hs.
+  rewrite seed_lookup. simpl.
+  rewrite isptr_offset_val_zero by exact Hptr.
+  change (s = s). reflexivity.
+Qed.
+
+Lemma seed_store_v64_eval : forall Delta c0 x s,
+  ENTAIL Delta,
+    PROP () LOCAL (temp _s s; temp _c (Vlong x))
+    SEP (seed_data_v64 Ews c0 s) |--
+    local (fun rho => Vlong x =
+      eval_expr (Ecast seed_store_v64_value tulong) rho).
+Proof.
+  intros. unfold seed_store_v64_value.
+  apply andp_left2. intro rho.
+  unfold PROPx, LOCALx, SEPx. simpl.
+  unfold local, lift1. unfold_lift. simpl.
+  constructor. intros w H.
+  destruct H as [_ Hrest]. simpl in Hrest |- *.
+  destruct Hrest as [Hlocals _].
+  destruct Hlocals as [_ [[Hx _] _]].
+  rewrite <- Hx. change (Vlong x = Vlong x). reflexivity.
+Qed.
+
+Lemma exact_seed_load_v32_address : forall Delta x s,
+  ENTAIL Delta,
+    PROP () LOCAL (temp _s s; temp _c (Vlong x))
+    SEP (exact_seed_v64 Ews x s) |--
+    local (fun rho => s = eval_lvalue seed_load_v32_expr rho).
+Proof.
+  intros Delta x s.
+  unfold seed_load_v32_expr.
+  apply andp_left2. intro rho.
+  unfold PROPx, LOCALx, SEPx. simpl.
+  unfold local, lift1. unfold_lift. simpl.
+  constructor. intros w H.
+  destruct H as [Hlocal Hexact].
+  simpl in Hexact |- *.
+  destruct Hexact as [Hlocals Hsep].
+  destruct Hlocals as [[Hs _] _].
+  destruct Hsep as [w1 [w2 [_ [Hseed _]]]].
+  destruct Hseed as [Hfc _].
+  destruct Hfc as [Hptr _].
+  rewrite <- Hs.
+  rewrite seed_lookup. simpl.
+  rewrite isptr_offset_val_zero by exact Hptr.
+  change (s = s). reflexivity.
+Qed.
+
+Lemma seed_v64_store_ramify : forall c0 x s,
+  seed_data_v64 Ews c0 s |--
+    mapsto_ Ews tulong s *
+      (exact_mapsto Ews Mint64 (Vlong x) s -* exact_seed_v64 Ews x s).
+Proof.
+  intros c0 x s.
+  unfold seed_data_v64.
+  unfold data_at, field_at, at_offset, offset_val.
+  simpl; rewrite data_at_rec_eq; simpl.
+  unfold exact_seed_type in *.
+  (* Generalize the dependent value before rewriting the composite lookup. *)
+  generalize (seed_value_shape c0).
+  generalize (unfold_reptype (seed_value c0)).
+  unfold reptype_unionlist, get_co.
+  rewrite seed_lookup. simpl.
+  intros v Hv. apply JMeq_eq in Hv. subst v.
+  unfold union_pred; simpl.
+  unfold withspacer, spacer.
+  destruct (Z.eq_dec (8 - 8) 0); [| lia].
+  lazymatch goal with
+  | |- context [data_at_rec Ews tulong (Vlong c0) ?p] =>
+      change (data_at_rec Ews tulong (Vlong c0) p)
+        with (mapsto Ews tulong p (Vlong c0))
+  end.
+  change (match s with
+          | Vptr b z => Vptr b (Ptrofs.add z (Ptrofs.repr 0))
+          | _ => Vundef end) with (offset_val 0 s).
+  rewrite <- (mapsto_offset_zero Ews tulong s (Vlong c0)).
+  unfold exact_seed_v64.
+  apply RAMIF_PLAIN.solve with
+    (F := !! field_compatible exact_seed_type [] s && emp).
+  - rewrite sepcon_andp_prop, sepcon_emp.
+    apply andp_derives; [apply derives_refl |].
+    apply mapsto_mapsto_.
+  - rewrite sepcon_andp_prop', emp_sepcon.
+    apply derives_refl.
+Qed.
+
+(* Instantiate semax_load_nth_ram using exact_Mint64_has_low32_mapsto_le.
+   The exact 8-byte predicate remains in SEP, so repeated low-word loads do
+   not forget the high word. *)
+Lemma semax_seed_load_v32_exact :
+  forall {Espec : OracleKind} (Delta : tycontext)
+    (x : int64) (s : val) (k : statement) (Post : ret_assert),
+    typeof_temp Delta _t'1 = Some tuint ->
+    ENTAIL Delta,
+      PROP () LOCAL (temp _s s; temp _c (Vlong x))
+      SEP (exact_seed_v64 Ews x s) |--
+      (tc_lvalue Delta seed_load_v32_expr) &&
+      local (fun _ => tc_val tuint (Vint (Int64.loword x))) ->
+    semax Delta
+      (PROP ()
+       LOCAL (temp _t'1 (Vint (Int64.loword x));
+              temp _s s; temp _c (Vlong x))
+       SEP (exact_seed_v64 Ews x s))
+      k Post ->
+    semax Delta
+      (PROP ()
+       LOCAL (temp _s s; temp _c (Vlong x))
+      SEP (exact_seed_v64 Ews x s))
+      (Ssequence seed_load_v32_statement k) Post.
+Proof.
+  intros Espec Delta x s k Post Htemp Htc Hk.
+  eapply semax_seq'; [| exact Hk].
+  unfold seed_load_v32_statement.
+  eapply semax_pre0; [apply now_later |].
+  eapply semax_load_nth_ram with
+    (n := 0%nat) (sh := Ews) (Pre := exact_seed_v64 Ews x s)
+    (p := s) (v := Vint (Int64.loword x)) (t1 := tuint) (t2 := tuint).
+  - reflexivity.
+  - exact Htemp.
+  - reflexivity.
+  - apply exact_seed_load_v32_address.
+  - reflexivity.
+  - auto.
+  - unfold exact_seed_v64. apply andp_left2.
+    apply exact_Mint64_has_low32_mapsto_le.
+    + reflexivity.
+    + auto.
+  - exact Htc.
+Qed.
+
+End SeedSupport.
