fusion/tests/union_exact_view.v
@@ -1,0 +1,275 @@
+(* Proved exact-memory compatibility layer for narrowing integer reads. *)
+
+Require Import VST.floyd.proofauto.
+Require Import VST.floyd.library.
+Require Import VST.floyd.loadstore_mapsto.
+Require Import compcert.common.Memdata.
+Require Export VST.floyd.FusionExact.
+
+Local Open Scope Z.
+Local Open Scope logic.
+
+Definition address_memvals_at
+    (sh : share) (bl : list memval) (a : address) : mpred :=
+  predicates_hered.allp
+    (res_predicates.jam
+      (adr_range_dec a (Zlength bl))
+      (fun loc =>
+        res_predicates.yesat compcert_rmaps.RML.R.NoneP
+          (compcert_rmaps.VAL
+            (nth (Z.to_nat (snd loc - snd a)) bl Undef)) sh loc)
+      res_predicates.noat).
+
+Lemma address_memvals_at_app : forall sh bl1 bl2 b ofs,
+  address_memvals_at sh (bl1 ++ bl2) (b, ofs) =
+    address_memvals_at sh bl1 (b, ofs) *
+    address_memvals_at sh bl2 (b, ofs + Zlength bl1).
+Proof.
+  intros.
+  pose proof (Zlength_nonneg bl1) as Hlen1.
+  pose proof (Zlength_nonneg bl2) as Hlen2.
+  unfold address_memvals_at.
+  simpl fst; simpl snd.
+  apply res_predicates.allp_jam_split2.
+  - eexists; apply res_predicates.is_resource_pred_YES_VAL'.
+  - eexists; apply res_predicates.is_resource_pred_YES_VAL'.
+  - eexists; apply res_predicates.is_resource_pred_YES_VAL'.
+  - rewrite Zlength_app. split; intros [b' z]; unfold adr_range; simpl.
+    + split.
+      * intros [Hb Hz]. subst b'.
+        destruct (Z_lt_ge_dec z (ofs + Zlength bl1)).
+        -- left; split; auto; lia.
+        -- right; split; auto; lia.
+      * intros [[Hb Hz] | [Hb Hz]]; subst b'; split; auto; lia.
+    + intros [_ Hz1] [_ Hz2]. lia.
+  - intros [b' z] Hrange. unfold adr_range in Hrange. simpl in Hrange.
+    destruct Hrange as [-> Hz]. simpl.
+    f_equal. f_equal.
+    rewrite app_nth1; auto.
+    rewrite <- ZtoNat_Zlength.
+    apply Z2Nat.inj_lt; lia.
+  - intros [b' z] Hrange. unfold adr_range in Hrange. simpl in Hrange.
+    destruct Hrange as [-> Hz]. simpl.
+    f_equal. f_equal.
+    rewrite app_nth2.
+    + f_equal.
+      apply Nat2Z.inj.
+      rewrite Nat2Z.inj_sub.
+      * rewrite !Z2Nat.id by lia.
+        rewrite <- Zlength_correct.
+        lia.
+      * rewrite <- ZtoNat_Zlength.
+        apply Z2Nat.inj_le; lia.
+    + rewrite <- ZtoNat_Zlength.
+      apply Z2Nat.inj_le; lia.
+  - intros loc m sh' k Hrange Hyes Hoption.
+    left.
+    destruct Hyes as [rsh Hyes].
+    unfold res_predicates.yesat_raw in Hyes.
+    rewrite Hyes in Hoption.
+    inversion Hoption; exact I.
+Qed.
+
+Lemma exact_address_mapsto_memvals : forall sh ch v a,
+  exact_address_mapsto sh ch v a =
+    !! (align_chunk ch | snd a) &&
+    address_memvals_at sh (encode_val ch v) a.
+Proof.
+  intros.
+  unfold exact_address_mapsto, res_predicates.address_mapsto_old,
+    address_memvals_at, res_predicates.nthbyte.
+  rewrite Zlength_correct, encode_val_length, <- size_chunk_conv.
+  reflexivity.
+Qed.
+
+Lemma address_memvals_at_to_address_mapsto : forall sh ch v a,
+  (align_chunk ch | snd a) ->
+  address_memvals_at sh (encode_val ch v) a |--
+    res_predicates.address_mapsto ch
+      (decode_val ch (encode_val ch v)) sh a.
+Proof.
+  intros sh ch v a Halign.
+  constructor.
+  unfold address_memvals_at, res_predicates.address_mapsto.
+  rewrite Zlength_correct, encode_val_length, <- size_chunk_conv.
+  intros w Hw.
+  exists (encode_val ch v).
+  split.
+  - split3; auto using encode_val_length.
+  - exact Hw.
+Qed.
+
+Definition memvals_at (sh : share) (bl : list memval) (p : val) : mpred :=
+  match p with
+  | Vptr b ofs => address_memvals_at sh bl (b, Ptrofs.unsigned ofs)
+  | _ => FF
+  end.
+
+Definition pointer_aligned (ch : memory_chunk) (p : val) : Prop :=
+  match p with
+  | Vptr _ ofs => (align_chunk ch | Ptrofs.unsigned ofs)
+  | _ => False
+  end.
+
+Definition pointer_offset (p : val) : Z :=
+  match p with Vptr _ ofs => Ptrofs.unsigned ofs | _ => 0 end.
+
+(* The split pointer, including an empty suffix, must not wrap. *)
+Lemma memvals_at_app : forall sh bl1 bl2 p,
+  isptr p ->
+  0 <= pointer_offset p + Zlength bl1 <= Ptrofs.max_unsigned ->
+  memvals_at sh (bl1 ++ bl2) p =
+    memvals_at sh bl1 p * memvals_at sh bl2 (offset_val (Zlength bl1) p).
+Proof.
+  intros sh bl1 bl2 p Hp Hr.
+  destruct p; try contradiction.
+  unfold memvals_at, offset_val; simpl in *.
+  pose proof (Ptrofs.unsigned_range i).
+  pose proof (Zlength_nonneg bl1).
+  rewrite Ptrofs.add_unsigned.
+  rewrite (Ptrofs.unsigned_repr (Zlength bl1)) by lia.
+  rewrite Ptrofs.unsigned_repr by exact Hr.
+  apply address_memvals_at_app.
+Qed.
+
+Lemma exact_mapsto_memvals : forall sh ch v p,
+  isptr p ->
+  exact_mapsto sh ch v p =
+    !! pointer_aligned ch p && memvals_at sh (encode_val ch v) p.
+Proof.
+  intros sh ch v p Hp. destruct p; try contradiction.
+  apply exact_address_mapsto_memvals.
+Qed.
+
+Lemma memvals_Mint32_has_mapsto : forall sh x p,
+  readable_share sh -> pointer_aligned Mint32 p ->
+  memvals_at sh (encode_val Mint32 (Vint x)) p |-- mapsto sh tuint p (Vint x).
+Proof.
+  intros sh x p Hread HA. destruct p; try contradiction.
+  unfold memvals_at, mapsto; simpl.
+  destruct (readable_share_dec sh); [| contradiction].
+  apply orp_right1, andp_right; [apply prop_right; exact I |].
+  replace (Vint x) with (decode_val Mint32 (encode_val Mint32 (Vint x))).
+  - apply (address_memvals_at_to_address_mapsto sh Mint32 (Vint x)
+      (b, Ptrofs.unsigned i)); exact HA.
+  - unfold encode_val, decode_val. rewrite proj_inj_bytes.
+    f_equal. apply decode_encode_int_4.
+Qed.
+
+(* Specialize Memdata.bytes_of_int64 to Vlong and little-endian targets. *)
+Lemma encode_val_Mint64_Vlong_split_le :
+  Archi.big_endian = false ->
+  forall x,
+    encode_val Mint64 (Vlong x) =
+      encode_val Mint32 (Vint (Int64.loword x)) ++
+      encode_val Mint32 (Vint (Int64.hiword x)).
+Proof.
+  intros Hle x.
+  unfold encode_val, inj_bytes.
+  rewrite <- map_app.
+  f_equal.
+  unfold encode_int, rev_if_be.
+  rewrite Hle.
+  apply bytes_of_int64.
+Qed.
+
+(* A prefix projection needs no representable pointer to the unused suffix. *)
+Lemma memvals_at_prefix : forall sh bl1 bl2 p,
+  memvals_at sh (bl1 ++ bl2) p |-- memvals_at sh bl1 p * TT.
+Proof.
+  intros. destruct p; try apply FF_left.
+  unfold memvals_at. rewrite address_memvals_at_app.
+  apply sepcon_derives; [apply derives_refl | apply TT_right].
+Qed.
+
+(* Keep the shipped low-word interface free of an unnecessary p+4 bound. *)
+Lemma exact_Mint64_has_low32_mapsto_le : forall sh x p,
+  Archi.big_endian = false ->
+  readable_share sh ->
+  exact_mapsto sh Mint64 (Vlong x) p |--
+    mapsto sh tuint p (Vint (Int64.loword x)) * TT.
+Proof.
+  intros sh x p Hle Hread.
+  destruct p as [| | | | |b ofs]; try apply FF_left.
+  rewrite exact_mapsto_memvals by exact I.
+  apply derives_extract_prop; intro Halign.
+  rewrite (encode_val_Mint64_Vlong_split_le Hle x).
+  eapply derives_trans; [apply memvals_at_prefix |].
+  apply sepcon_derives; [| apply derives_refl].
+  apply (memvals_Mint32_has_mapsto sh (Int64.loword x) (Vptr b ofs) Hread).
+  simpl in Halign |- *. destruct Halign as [k Hk].
+  refine (ex_intro _ (2 * k)%Z _). lia.
+Qed.
+
+(* Retaining Mint64 alignment is essential for the reverse direction. *)
+Lemma exact_Mint64_split32_le : forall sh x p,
+  Archi.big_endian = false -> isptr p ->
+  0 <= pointer_offset p + 4 <= Ptrofs.max_unsigned ->
+  exact_mapsto sh Mint64 (Vlong x) p =
+    !! pointer_aligned Mint64 p &&
+    (exact_mapsto sh Mint32 (Vint (Int64.loword x)) p *
+     exact_mapsto sh Mint32 (Vint (Int64.hiword x)) (offset_val 4 p)).
+Proof.
+  intros sh x p Hle Hp Hr. destruct p; try contradiction.
+  unfold exact_mapsto, offset_val, pointer_aligned; simpl in *.
+  rewrite Ptrofs.add_unsigned.
+  rewrite (Ptrofs.unsigned_repr 4) by computable.
+  rewrite Ptrofs.unsigned_repr by exact Hr.
+  rewrite !exact_address_mapsto_memvals.
+  rewrite (encode_val_Mint64_Vlong_split_le Hle x), address_memvals_at_app.
+  change (Zlength (encode_val Mint32 (Vint (Int64.loword x)))) with 4.
+  rewrite sepcon_andp_prop, sepcon_andp_prop'.
+  apply pred_ext; entailer!.
+  simpl in H |- *. destruct H as [k Hk]. split; first
+    [refine (ex_intro _ (2 * k)%Z _); lia
+    | refine (ex_intro _ (2 * k + 1)%Z _); lia].
+Qed.
+
+Lemma exact_Mint32_has_mapsto : forall sh x p,
+  readable_share sh ->
+  exact_mapsto sh Mint32 (Vint x) p |-- mapsto sh tuint p (Vint x).
+Proof.
+  intros sh x p Hread. destruct p; try apply FF_left.
+  rewrite exact_mapsto_memvals by exact I.
+  apply derives_extract_prop; intro HA.
+  apply memvals_Mint32_has_mapsto; assumption.
+Qed.
+
+Lemma exact_Mint64_has_high32_mapsto_le : forall sh x p,
+  Archi.big_endian = false -> readable_share sh -> isptr p ->
+  0 <= pointer_offset p + 4 <= Ptrofs.max_unsigned ->
+  exact_mapsto sh Mint64 (Vlong x) p |--
+    mapsto sh tuint (offset_val 4 p) (Vint (Int64.hiword x)) * TT.
+Proof.
+  intros sh x p Hle Hread Hp Hr.
+  rewrite exact_Mint64_split32_le by assumption.
+  apply andp_left2. rewrite sepcon_comm.
+  apply sepcon_derives; [apply exact_Mint32_has_mapsto; assumption | apply TT_right].
+Qed.
+
+Lemma exact_Mint64_has_mapsto : forall sh x p,
+  readable_share sh ->
+  exact_mapsto sh Mint64 (Vlong x) p |-- mapsto sh tulong p (Vlong x).
+Proof.
+  intros sh x p Hread.
+  destruct p as [| | | | |b ofs]; try apply FF_left.
+  unfold exact_mapsto. rewrite exact_address_mapsto_memvals.
+  apply derives_extract_prop; intro HA.
+  unfold mapsto; simpl.
+  destruct (readable_share_dec sh); [| contradiction].
+  apply orp_right1, andp_right; [apply prop_right; exact I |].
+  replace (Vlong x) with (decode_val Mint64 (encode_val Mint64 (Vlong x))).
+  - apply (address_memvals_at_to_address_mapsto sh Mint64 (Vlong x)
+      (b, Ptrofs.unsigned ofs)); exact HA.
+  - unfold encode_val, decode_val. rewrite proj_inj_bytes.
+    f_equal. apply decode_encode_int_8.
+Qed.
+
+Lemma exact_Mint64_has_full_mapsto_frame : forall sh x p,
+  readable_share sh ->
+  exact_mapsto sh Mint64 (Vlong x) p |-- mapsto sh tulong p (Vlong x) * TT.
+Proof.
+  intros. eapply derives_trans; [apply exact_Mint64_has_mapsto; assumption |].
+  rewrite <- (sepcon_emp (mapsto sh tulong p (Vlong x))) at 1.
+  apply sepcon_derives; [apply derives_refl | apply TT_right].
+Qed.
