fusion/tests/verif_fusion.v
@@ -1,0 +1,140 @@
+Require Import VST.floyd.proofauto.
+Require Import seed_program union_exact_seed_interface union_exact_seed_spec fusion_store.
+Import compcert.lib.Maps.
+Local Open Scope logic.
+
+Module ProgramLayout <: SEED_LAYOUT.
+#[export] Instance CompSpecs : compspecs. make_compspecs prog. Defined.
+Lemma seed_lookup : PTree.get seed_union_rw._seed cenv_cs = Some SeedReference.seed_composite.
+Proof. reflexivity. Qed.
+Definition seed_value (x : int64) : reptype (Tunion seed_union_rw._seed noattr) := inr (Vlong x).
+Lemma seed_value_shape : forall x,
+  JMeq (unfold_reptype (seed_value x)) (inr (Vlong x) : val + val).
+Proof. intros; exact (unfold_reptype_JMeq _ (seed_value x)). Qed.
+End ProgramLayout.
+#[export] Instance CompSpecs : compspecs := ProgramLayout.CompSpecs.
+Definition Vprog : varspecs. mk_varspecs prog. Defined.
+Include SeedSpec ProgramLayout.
+
+Definition exact_spec := w64_r32_exact_spec.
+Definition caller_spec : ident * funspec :=
+  DECLARE _mixed_caller
+  WITH c0 : int64, x : int64, s : val
+  PRE [tptr tseed_exact, tulong]
+    PROP () PARAMS (s; Vlong x)
+    SEP (data_at Ews tseed_exact (inr (Vlong c0)) s)
+  POST [tuint]
+    PROP () RETURN (Vint (Int64.loword x))
+    SEP (seed_v64_exact Ews x s).
+Definition main_spec :=
+  DECLARE _main
+  WITH gv : globals
+  PRE [] main_pre prog tt gv
+  POST [tint] main_post prog gv.
+Definition Gprog : funspecs := [exact_spec; caller_spec; main_spec].
+
+Lemma body_w64_r32 : semax_body Vprog Gprog f_w64_r32 exact_spec.
+Proof.
+  start_function.
+  change (fn_body f_w64_r32) with
+    (Ssequence seed_store_v64_statement
+      (Ssequence seed_load_v32_statement (Sreturn (Some (Etempvar _t'1 tuint))))).
+  eapply semax_seq' with (P' :=
+    PROP () LOCAL (temp _s s; temp _c (Vlong x))
+    SEP (exact_seed_v64 Ews x s)).
+  - unfold seed_store_v64_statement.
+    eapply semax_pre0; [apply now_later |].
+    eapply semax_store_exact_nth_ram with
+      (n := 0%nat) (Pre := seed_data_v64 Ews c0 s)
+      (R := [seed_data_v64 Ews c0 s]) (Post := exact_seed_v64 Ews x s)
+      (p := s) (v := Vlong x) (sh := Ews) (t1 := tulong) (ch := Mint64).
+    + reflexivity.
+    + reflexivity.
+    + apply seed_store_v64_address.
+    + apply seed_store_v64_eval.
+    + reflexivity.
+    + auto.
+    + apply seed_v64_store_ramify.
+    + unfold seed_store_v64_lvalue, seed_store_v64_value, seed_data_v64.
+      entailer!.
+  - eapply semax_seed_load_v32_exact.
+    + reflexivity.
+    + unfold seed_load_v32_expr.
+      sep_apply exact_seed_v64_isptr. entailer!.
+    + forward.
+Qed.
+
+Lemma seed_initializer sh x p :
+  data_at sh tulong (Vlong x) p =
+  data_at sh tseed_exact (inr (Vlong x)) p.
+Proof.
+  assert (HA : align_compatible tulong p = align_compatible tseed_exact p).
+  { unfold align_compatible. destruct p; try reflexivity.
+    apply prop_ext; split; intro H.
+    - eapply align_compatible_rec_Tunion with (co := get_co _seed).
+      + reflexivity.
+      + reflexivity.
+      + intros id t Ht. simpl in Ht.
+        destruct (ident_eq id _v32).
+        * inversion Ht; subst.
+          eapply align_compatible_rec_by_value; [reflexivity |].
+          pose proof (align_compatible_rec_by_value_inv _ tulong Mint64 _ eq_refl H) as HD.
+          change (8 | Ptrofs.unsigned i) in HD.
+          change (4 | Ptrofs.unsigned i).
+          destruct HD as [k Hk]; exists (2*k)%Z; lia.
+        * destruct (ident_eq id _v64); inversion Ht; subst; exact H.
+    - exact (align_compatible_rec_Tunion_inv cenv_cs _seed noattr (get_co _seed)
+        _ eq_refl H _v64 tulong eq_refl). }
+  unfold data_at, field_at, at_offset, offset_val.
+  simpl; rewrite (data_at_rec_eq sh tseed_exact); simpl; unfold union_pred; simpl.
+  unfold field_compatible. rewrite <- HA.
+  unfold size_compatible; simpl.
+  unfold withspacer, spacer.
+  destruct (Z.eq_dec (8 - 8) 0); [| lia].
+  reflexivity.
+Qed.
+
+Lemma body_caller : semax_body Vprog Gprog f_mixed_caller caller_spec.
+Proof. start_function. forward_call (c0, x, s). forward. Qed.
+
+Lemma body_main : semax_body Vprog Gprog f_main main_spec.
+Proof.
+  start_function.
+  rewrite seed_initializer.
+  forward_call (Int64.zero, Int64.repr 4294967338, gv _global_seed).
+  forward.
+Qed.
+
+(* The pre-existing forward store keeps its ordinary data_at postcondition. *)
+Lemma ordinary_forward_store_regression : forall {Espec : OracleKind} c0 x s,
+  semax (func_tycontext f_w64_r32 Vprog Gprog nil)
+    (PROP () LOCAL (temp _s s; temp _c (Vlong x))
+     SEP (data_at Ews tseed_exact (inr (Vlong c0)) s))
+    seed_store_v64_statement
+    (normal_ret_assert
+      (PROP () LOCAL (temp _s s; temp _c (Vlong x))
+       SEP (data_at Ews tseed_exact (inr (Vlong x)) s))).
+Proof.
+  intros.
+  unfold seed_store_v64_statement, seed_store_v64_lvalue, seed_store_v64_value.
+  forward.
+  entailer!.
+Qed.
+
+Require Import VST.floyd.VSU.
+
+Definition seedVSU : @VSU NullExtension.Espec [] []
+  ltac:(QPprog prog) Gprog (InitGPred (Vardefs ltac:(QPprog prog))).
+Proof.
+  mkVSU prog Gprog.
+  - solve_SF_internal body_w64_r32.
+  - solve_SF_internal body_caller.
+  - solve_SF_internal body_main.
+Qed.
+
+Print Assumptions semax_store_exact_nth_ram.
+Print Assumptions body_w64_r32.
+Print Assumptions body_caller.
+Print Assumptions body_main.
+Print Assumptions ordinary_forward_store_regression.
+Print Assumptions seedVSU.
