Makefile
@@ -523,6 +523,7 @@ ZLIST_FILES= \
   sublist.v Zlength_solver.v list_solver.v
 
 FLOYD_FILES= \
+   FusionExact.v FusionExactSem.v FusionStore.v \
    coqlib3.v base.v seplog_tactics.v typecheck_lemmas.v val_lemmas.v assert_lemmas.v find_nth_tactic.v const_only_eval.v \
    base2.v functional_base.v go_lower.v \
    library.v proofauto.v computable_theorems.v computable_functions.v \
@@ -714,7 +715,7 @@ else
 PROGS_FILES=$(PROGS32_FILES)
 endif
 
-INSTALL_FILES_SRC=$(shell COMPCERT=$(COMPCERT) COMPCERT_INST_DIR=$(COMPCERT_INST_DIR) ZLIST=$(ZLIST) BITSIZE=$(BITSIZE) ARCH=$(ARCH) IGNORECOQVERSION=$(IGNORECOQVERSION) IGNORECOMPCERTVERSION=$(IGNORECOMPCERTVERSION) MAKE=$(MAKE) util/calc_install_files $(PROGSDIR))
+INSTALL_FILES_SRC=$(shell COMPCERT=$(COMPCERT) COMPCERT_INST_DIR=$(COMPCERT_INST_DIR) ZLIST=$(ZLIST) BITSIZE=$(BITSIZE) ARCH=$(ARCH) IGNORECOQVERSION=$(IGNORECOQVERSION) IGNORECOMPCERTVERSION=$(IGNORECOMPCERTVERSION) MAKE=$(MAKE) util/calc_install_files '$(PROGSDIR) simpleconc')
 INSTALL_FILES_VO=$(patsubst %.v,%.vo,$(INSTALL_FILES_SRC))
 INSTALL_FILES=$(sort $(INSTALL_FILES_SRC) $(INSTALL_FILES_VO))
 
@@ -1002,4 +1003,3 @@ assumptions.txt: veric/tcb.vo
 # such problem, not sure exactly.  -- Andrew)
 include .depend
 -include .depend-concur
-
